o not much

checker/checker.v
@@ -1555,216 +1555,261 @@ Inductive step : Type :=
    H, x : A, J |- A
  *)
 | step_assumption  (x : HName)                                : step
+
 (*
        H, J |- B
    ---------------- (clear x)
    H, x : A, J |- B
  *)
 | step_clear       (x : HName)                                : step
+
 (*
    H, x : A |- B
    ------------- (imply_right x)
     H |- A -> B
  *)
 | step_imply_right (x : HName)                                : step
+
 (*
    H, J |- A      H, x : B, J |- C
    ------------------------------- (imply_left x)
        H, x : A -> B, J |- C
  *)
 | step_imply_left  (x : HName)                                : step
+
 (*
    H, x : A, J |- C      H, x : B, J |- C
    -------------------------------------- (or_left x)
              H, x : A \/ B, J |- C
  *)
 | step_or_left     (x : HName)                                : step
+
 (*
    H, x : A, y : B, J |- C
    ----------------------- (and_left x y)
     H, x : A /\ B, J |- C
  *)
 | step_and_left    (x y : HName)                              : step
+
 (*
    H, x : A -> B, y : B -> A, J |- C
    ----------------------- (equiv_left x y)
     H, x : A <-> B, J |- C
  *)
 | step_equiv_left  (x y : HName)                              : step
+
 (*
    H |- A -> B      H |- B -> A
    ---------------------------- (equiv_right)
           H |- A <-> B
  *)
 | step_equiv_right                                            : step
+
 (*
    H |- A      H |- B
    ------------------ (and_right)
       H |- A /\ B
  *)
 | step_and_right                                              : step
+
 (*
      H |- A
    ----------- (or_right1)
    H |- A \/ B
  *)
 | step_or_right1                                              : step
+
 (*
      H |- B
    ----------- (or_right2)
    H |- A \/ B
  *)
 | step_or_right2                                              : step
+
 (*
           H, J |- A
    --------------------- (not_left x)
    H, x : not(A), J |- C
  *)
 | step_not_left    (x : HName)                                : step
+
 (*
    H, x : A |- False
    ----------------- (not_right x)
       H |- not(A)
  *)
 | step_not_right   (x : HName)                                : step
+
 (*
    H, J, x : A, y : B, K |- C
    -------------------------- (move_hyp)
    H, x : A, J, y : B, K |- C
  *)
 | step_move_hyp    (x y : HName)                              : step
+
 (*
    H |- f      H, x : f |- A
    ------------------------- (cut x f)
              H |- A
  *)
 | step_cut         (x : HName) (f : Formula)                  : step
+
 (*
    H, x : sw(sub(DI_ge_axiom)) |- A
    -------------------------------- (DIge x sub sw)
                H |- A
  *)
 | step_DIge        (x : HName) (sub : US) (sw : SW)           : step
+
 (*
    H, x : sw(sub(DI_ge_diff_axiom)) |- A
    ------------------------------------- (DIgeD x sub sw)
                 H |- A
  *)
 | step_DIgeD       (x : HName) (sub : US) (sw : SW)           : step
+
 (*
    H, x : sw(sub(ode_comm)) |- A
    ----------------------------- (OC x sub sw)
             H |- A
  *)
 | step_OC          (x : HName) (sub : US) (sw : SW)           : step
+
 (*
    H, x : sw(sub(DG_LR_axiom)) |- A
    -------------------------------- (DGhostLR x sub sw)
               H |- A
  *)
 | step_DGhostLR    (x : HName) (sub : US) (sw : SW)           : step
+
 (*
    H, x : sw(sub(sp_DG_LR_axiom)) |- A
    ----------------------------------- (spDGhostLR x sub sw)
                 H |- A
  *)
 | step_spDGhostLR  (x : HName) (sub : US) (sw : SW)           : step
+
 (*
    H, x : sw(differential_identity_axiom) |- A
    ------------------------------------------- (XP x sw)
                     H |- A
  *)
 | step_XP          (x : HName) (sw : SW)                      : step
+
 (*
    H, x : sw(sub(pred_XP_axiom)) |- A
    ---------------------------------- (PXP x sub sw)
                H |- A
  *)
 | step_PXP         (x : HName) (sub : US) (sw : SW)           : step
+
 (*
    H, x : sw(sub(quant_pred_XP_axiom)) |- A
    ---------------------------------------- (QPXP x sub sw)
                   H |- A
  *)
 | step_QPXP        (x : HName) (sub : US) (sw : SW)           : step
+
 (*
    H, x : sw(sub(differential_effect_axiom)) |- A
    ---------------------------------------------- (DE x sub sw)
                       H |- A
  *)
 | step_DE          (x : HName) (sub : US) (sw : SW)           : step
+
 (*
    H, x : sw(sub(differential_effect_sch_axiom v t ode Q P)) |- A
    -------------------------------------------------------------- (DEsch x v t ode Q P)
                               H |- A
  *)
 | step_DEsch       (x : HName) (v : Var) (t : Term) (ode : ODE) (Q P : Formula) : step
+
 (*
    H, x : sub(V_axiom) |- A
    ------------------------ (V x sub)
            H |- A
  *)
 | step_V           (x : HName) (sub : US)                     : step
+
 (*
    H, x : sub(diff_real_axiom r) |- A
    ---------------------------------- (DR x sub sw r)
               H |- A
  *)
 | step_DR          (x : HName) (sub : US) (sw : SW) (r : R)   : step
+
 (*
    H, x : sub(diff_realn_axiom r) |- A
    ----------------------------------- (DRN x sub sw r)
                 H |- A
  *)
 | step_DRN         (x : HName) (sub : US) (sw : SW) (r : nat) : step
+
 (*
    ∅ |- sub(Q)      H, x : sub([a]Q) |- A
    --------------------------------------- (G x sub)
                     H |- A
  *)
 | step_G           (x : HName) (sub : US)                     : step
+
 (*
    H, x : sw(sub(assignment_axiom)) |- A
    ------------------------------------- (assign x sub sw)
                 H |- A
  *)
 | step_assign      (x : HName) (sub : US) (sw : SW)           : step
+
 (*
    H, x : sw(sub(assignmentp_axiom)) |- A
    -------------------------------------- (assignp x sub sw)
                 H |- A
  *)
 | step_assignp     (x : HName) (sub : US) (sw : SW)           : step
+
 (*
    H, x : sub(K_quant_axiom) |- A
    ------------------------------ (K x sub)
                 H |- A
  *)
 | step_K           (x : HName) (sub : US)                     : step
+
 (*
    ∅ |- P <-> Q      H, x : [qsC -> C](qC P <> qC Q) |- A
    ------------------------------------------------------ (CE x P Q C)
                 H |- A
  *)
 | step_CE          (x : HName) (P Q C : Formula)              : step
+
 (*
    H |- t > u
    ---------- (GE2GT)
    H |- t ≥ u
  *)
 | step_GE2GT                                                  : step
+
 (*
              ∅
-   -------------------- (false_left)
+   -------------------- (false_left x)
    H, x : False, J |- C
  *)
 | step_false_left (x : HName)                                 : step
+
+(*
+(*
+     H |- p(y)
+   ------------- (all_right y)
+   H |- ∀x.p(x)
+ *)
+| step_all_right (y : KVariable)                              : step
+*)
+
 (*
    sw(H |- A)
    ---------- (swap sw)
     H |- A
  *)
 | step_swap        (sw : swapping)                            : step
+
 | step_focus       (n : nat)                                  : step.
 (*| step_US          (sub : US)                : step*)
 
@@ -1806,6 +1851,7 @@ Ltac dstep h c :=
 (*  | Case_aux c "US"*)
   | Case_aux c "GE2GT"
   | Case_aux c "FalseLeft"
+(*  | Case_aux c "AllRight"*)
   | Case_aux c "Swap"
   | Case_aux c "Focus"
   ].
@@ -1914,6 +1960,16 @@ Proof.
   repeat introv; simpl.
   introv h1 h2 h3; tcsp.
 Qed.
+
+
+Fixpoint free_vars_hyp (h : hypothesis) : EAssignables :=
+  free_vars_formula (hyp_form h).
+
+Fixpoint free_vars_hyps (H : hypotheses) : EAssignables :=
+  match H with
+  | [] => FCS_finite []
+  | h :: hs => EAssignables_app (free_vars_hyp h) (free_vars_hyps hs)
+  end.
 
 
 Definition apply_step (ps : proof_state) (s : step) : proof_state :=
@@ -2218,6 +2274,21 @@ Definition apply_step (ps : proof_state) (s : step) : proof_state :=
       end
     | _ => ps
     end
+
+(*
+  | step_all_right y =>
+    match ps with
+    | MkSeq H C :: seqs =>
+      match C with
+      | KFforallVars [x] P =>
+        if in_eassignables y (free_vars_hyps H)
+        then ps
+        else (MkSeq H (swap_formula (MkSwapping x y) P)) :: seqs
+      | _ => ps
+      end
+    | _ => ps
+    end
+*)
 
   | step_swap sw =>
     match ps with
@@ -2601,6 +2672,25 @@ Proof.
   rewrite in_app_iff; rewrite in_snoc; tcsp.
 Qed.
 
+(*
+Lemma sequent_true_all_right :
+  forall H x y C,
+    in_eassignables y (free_vars_hyps H) = false
+    -> sequent_true (H ⊢ swap_formula (MkSwapping x y) C)
+    -> sequent_true (H ⊢ KFforallVars [x] C).
+Proof.
+  introv ie st hyps ers; simpl in *.
+  destruct rs; simpl in *; ginv.
+  destruct rs; simpl in *; ginv.
+  pose proof (st (swap_interp (MkSwapping x y) I) (swap_state (MkSwapping x y) (upd_state v x r))) as q; simpl in q.
+  unfold sequent_true_I_v, DSF in q; simpl in q.
+  rewrite <- swap_dynamic_semantics_formula2 in q.
+  apply q; clear q.
+  introv i.
+  applydup hyps in i as j; unfold DSF in j.
+Qed.
+*)
+
 Lemma apply_step_preserves_soundness :
   forall ps s,
     sound_proof_state (apply_step ps s)
@@ -2954,6 +3044,20 @@ Proof.
     apply find_hyp_some_implies in Heqfxh; subst.
     allrw sound_proof_state_cons; repnd; dands; auto.
     apply sequent_true_false_left. }
+
+  (*
+  { Case "AllRight".
+
+    destruct ps; simpl in *; auto.
+    destruct s as [H C]; simpl in *; auto.
+    destruct C; simpl in *; auto.
+    destruct vars; simpl in *; auto.
+    destruct vars; simpl in *; auto.
+    dest_cases w.
+    symmetry in Heqw.
+    allrw sound_proof_state_cons; repnd; dands; auto.
+    clear sound.
+  }*)
 
   { Case "Swap".
 
